Renaming types to begin with lowercase

src/AncillaHeap.fst
@@ -10,21 +10,21 @@ open Set
 open Total
 open PairHeap
 
-type AncHeapRecord = { hp:intHeap; max:int }
-type cond (ah:AncHeapRecord) = 
+type ancHeapRecord = { hp:intHeap; max:int }
+type cond (ah:ancHeapRecord) = 
   is_heap ah.hp /\ (forall i. (PairHeap.mem i ah.hp ==> i < ah.max))
 (* Correctness is encoded in the type *)
-type AncHeap = ah:AncHeapRecord{cond ah}
+type ancHeap = ah:ancHeapRecord{cond ah}
 
-val emptyHeap : AncHeap
-val above     : int -> Tot AncHeap
-val maxUsed   : AncHeap -> Tot int
-val dat       : AncHeap -> Tot intHeap
-val insert    : AncHeap -> int -> Tot AncHeap
-val popMin    : AncHeap -> Tot (AncHeap * int)
-val getn      : AncHeap -> nat -> Tot (AncHeap * list int)
-val getn_acc  : AncHeap -> (list int) -> n:nat -> Tot (AncHeap * list int) (decreases n)
-val mem       : int -> AncHeap -> Tot bool
+val emptyHeap : ancHeap
+val above     : int -> Tot ancHeap
+val maxUsed   : ancHeap -> Tot int
+val dat       : ancHeap -> Tot intHeap
+val insert    : ancHeap -> int -> Tot ancHeap
+val popMin    : ancHeap -> Tot (ancHeap * int)
+val getn      : ancHeap -> nat -> Tot (ancHeap * list int)
+val getn_acc  : ancHeap -> (list int) -> n:nat -> Tot (ancHeap * list int) (decreases n)
+val mem       : int -> ancHeap -> Tot bool
 
 let emptyHeap = { hp = Empty; max = 0 }
 let above n   = { hp = Empty; max = n }
@@ -53,61 +53,61 @@ let getn ah n = getn_acc ah [] n
 let mem i ah = if i >= ah.max then true else PairHeap.mem i ah.hp
 
 (** Verification utilities *)
-val elts      : AncHeap -> Tot (set int)
-val get_min    : AncHeap -> Tot int
-val delete_min : AncHeap -> Tot AncHeap
+val elts      : ancHeap -> Tot (set int)
+val get_min    : ancHeap -> Tot int
+val delete_min : ancHeap -> Tot ancHeap
 
 let get_min ah = snd (popMin ah)
 let delete_min ah = fst (popMin ah)
 let elts ah = fun i -> mem i ah
 
 (* Ancilla heaps with all zero values *)
-type zeroHeap (st:state) (ah:AncHeap) = 
+type zeroHeap (st:state) (ah:ancHeap) = 
   forall i. (mem i ah) ==> (lookup st i = false)
 
-val pop_is_zero : st:state -> ah:AncHeap ->
+val pop_is_zero : st:state -> ah:ancHeap ->
   Lemma (requires (zeroHeap st ah))
         (ensures (lookup st (snd (popMin ah)) = false)) 
   [SMTPat (lookup st (snd (popMin ah)))]
 let pop_is_zero st ah = ()
 
-val max_increasing : ah:AncHeap ->
+val max_increasing : ah:ancHeap ->
   Lemma (requires true)
         (ensures (fst (popMin ah)).max >= ah.max)
 let max_increasing ah = ()
 
-val pop_not_elt : ah:AncHeap ->
+val pop_not_elt : ah:ancHeap ->
   Lemma (not (mem (get_min ah) (delete_min ah)))
 let pop_not_elt ah = match ah.hp with
   | Empty -> ()
   | Heap (r, lst) -> deleteMin_not_in_heap ah.hp
 
-val pop_elt : ah:AncHeap ->
+val pop_elt : ah:ancHeap ->
   Lemma (mem (get_min ah) ah)
 let pop_elt ah = ()
 
-val pop_subset : ah:AncHeap ->
+val pop_subset : ah:ancHeap ->
   Lemma (subset (elts (delete_min ah)) (elts ah))
 let pop_subset ah = match ah.hp with
   | Empty -> ()
   | Heap (r, lst) -> mem_mergePairs lst
 
-val pop_proper_subset : ah:AncHeap ->
+val pop_proper_subset : ah:ancHeap ->
   Lemma (subset (elts (delete_min ah)) (elts ah) /\
          not (mem (get_min ah) (delete_min ah)))
 let pop_proper_subset ah = pop_not_elt ah; pop_subset ah
 
-val zeroHeap_subset : st:state -> ah:AncHeap -> ah':AncHeap ->
+val zeroHeap_subset : st:state -> ah:ancHeap -> ah':ancHeap ->
   Lemma (requires (zeroHeap st ah /\ subset (elts ah') (elts ah)))
         (ensures  (zeroHeap st ah'))
 let zeroHeap_subset st ah ah' = ()
 
-val zeroHeap_insert : st:state -> ah:AncHeap -> i:int ->
+val zeroHeap_insert : st:state -> ah:ancHeap -> i:int ->
   Lemma (requires (zeroHeap st ah /\ lookup st i = false))
         (ensures  (zeroHeap st (insert ah i)))
 let zeroHeap_insert st ah i = ()
 
-val zeroHeap_insert_list : st:state -> ah:AncHeap -> lst:list int ->
+val zeroHeap_insert_list : st:state -> ah:ancHeap -> lst:list int ->
   Lemma (requires (zeroHeap st ah /\ (forall i. List.mem i lst ==> lookup st i = false)))
         (ensures  (zeroHeap st (List.fold_leftT insert ah lst)))
   (decreases lst)
@@ -116,11 +116,11 @@ let rec zeroHeap_insert_list st ah lst = match lst with
   | x::xs -> zeroHeap_insert st ah x; zeroHeap_insert_list st (insert ah x) xs
 
 (*
-type PairHeap_mem (i:int) (ah:AncHeap) =
-  | Ge_max : i':int -> ah':AncHeap -> b:(i' >= ah'.max) -> PairHeap_mem i' ah'
-  | Mem_heap : i':int -> ah':AncHeap -> b:b2t (Heap.mem i ah.hp) -> PairHeap_mem i' ah'
+type PairHeap_mem (i:int) (ah:ancHeap) =
+  | Ge_max : i':int -> ah':ancHeap -> b:(i' >= ah'.max) -> PairHeap_mem i' ah'
+  | Mem_heap : i':int -> ah':ancHeap -> b:b2t (Heap.mem i ah.hp) -> PairHeap_mem i' ah'
 *)
 
-val elts_insert : ah:AncHeap -> i:int ->
+val elts_insert : ah:ancHeap -> i:int ->
   Lemma (subset (elts (insert ah i)) (ins i (elts ah)))
 let elts_insert ah i = ()
